Ground_PDDL_Exec_Imp/Ground_PDDL_Plan_TP_Reduction.thy
@@ -1,0 +1,5 @@
+theory Ground_PDDL_Plan_TP_Reduction
+  imports Ground_PDDL_Problem_TP_Reduction
+begin
+
+end
